
\begin{problem}
(a)
Give the exact formula (as a function of $n$) for the number of
times ``bingo" is printed by Algorithm~\textsc{BingoPrint} below.
First express it as a summation formula and justify it. Then simplify it to 
obtain a closed-form expression. Show your derivation.

\noindent
(b)
Give the asymptotic value of the
number of ``bingo"s using the $\Theta$-notation. Include a brief justification. You will need a formula
for the sum of consecutive squares that you can find on the internet.

\begin{tabbing}
aa \= aa \= aa \= aa \= aa \= aa \= \kill
\textbf{Algorithm} \textsc{BingoPrint} $(n: \mbox{\bf integer})$ \\
      \> \textbf{for} $i \leftarrow 1$ \textbf{to} $2n+1$
                         \textbf{do} \\
      \> \> \textbf{for} $j \leftarrow 1$ \textbf{to} $i^2+2i$ \textbf{do} \\
      \> \> \> print(``bingo")
\end{tabbing}
\end{problem}

\begin{solution}
(a) Each ``print" is treated as a single output. Therefore, the equation for each print is

\[ \sum\limits_{j=1}^{i^2 + 2i} 1 \]
When applied to the outer for loop, our equation becomes

\[ \sum\limits_{i=1}^{2n+1}\sum\limits_{j=1}^{i^2 + 2i} 1 \]

Expanded, the sum is

\[ \sum\limits_{i=1}^{2n+1} i^2 + 2i \]

\[ \sum\limits_{i=1}^{2n+1} i^2 +  \sum\limits_{i=1}^{2n+1} 2i \]

\[ \sum\limits_{i=1}^{2n+1} i^2 +  2\sum\limits_{i=1}^{2n+1} i\]

\[ \frac{(2n+1)(2n+2)(2(2n+1))}{6} + 2\frac{(2n+1)(2n+2)}{2} \]

\[ \frac{(2n+1)(2n+2)(2(2n+1))}{6} + (2n+1)(2n+2) \]

\[ \frac{(2n+1)(2n+2)(4n+2)}{6} + (2n+1)(2n+2) \]

(b) The right side of the equation has the highest degree of n. 

\[ (2n+1)(2n+2)(4n+2) = ~(n^3) \]

\[ \Theta (n^3) \]

\end{solution}
%%%%%%%%%%%%%%%%%%%%%%%%%%%%
